add the generation of all base types
git-svn-id: https://projects.brucker.ch/hol-testgen/svn/HOL-TestGen/trunk/hol-testgen@10535 3260e6d1-4efc-4170-b0a7-36055960796d

src/OCL_compiler_meta_UML.thy
@@ -67,8 +67,12 @@ record ocl_ty_class =       TyObj_name :: string
                             TyObj_ass_arity :: nat
                             TyObj_from :: ocl_ty_class_node
                             TyObj_to :: ocl_ty_class_node
-datatype ocl_ty =           OclTy_base_boolean
+datatype ocl_ty =           OclTy_base_void
+                          | OclTy_base_boolean
                           | OclTy_base_integer
+                          | OclTy_base_unlimitednatural
+                          | OclTy_base_real
+                          | OclTy_base_string
                           | OclTy_class ocl_ty_class
                           | OclTy_collection ocl_collection ocl_ty
                           | OclTy_raw string (* denoting raw HOL-type.*)
@@ -103,9 +107,12 @@ record ocl_association =        OclAss_type     :: ocl_association_type
                                                     \<times> string option (* role *)) list"
 datatype ocl_ass_class =        OclAssClass ocl_association ocl_class_raw
 
-datatype ocl_def_base = OclDefBase "string list"
+datatype ocl_def_base = OclDefInteger "string" (* integer digit *)
+                      | OclDefReal "string (* integer digit (left) *) \<times> string (* integer digit (right) *)"
+                      | OclDefString "string"
 
-datatype ocl_data_shallow_base = ShallB_str string
+datatype ocl_data_shallow_base = ShallB_term ocl_def_base
+                               | ShallB_str string (* binding *)
                                | ShallB_self internal_oid
 datatype ocl_data_shallow =      Shall_base ocl_data_shallow_base
                                | Shall_list "ocl_data_shallow_base list"
@@ -122,6 +129,8 @@ record ocl_instance_single = Inst_name :: string
                                            ocl_list_attr"
 
 datatype ocl_instance = OclInstance "ocl_instance_single list" (* mutual recursive *)
+
+datatype ocl_def_base_l = OclDefBase "ocl_def_base list"
 
 datatype 'a ocl_def_state_core = OclDefCoreAdd ocl_instance_single
                                | OclDefCoreSkip
@@ -309,22 +318,39 @@ definition "apply_optim_ass_arity ty_obj v =
    else Some v)"
 
 fun_quick str_of_ty where
-    "str_of_ty OclTy_base_boolean = ''Boolean''"
+    "str_of_ty OclTy_base_void = ''Void''"
+   |"str_of_ty OclTy_base_boolean = ''Boolean''"
    |"str_of_ty OclTy_base_integer = ''Integer''"
-   |"str_of_ty (OclTy_class ty_obj) = flatten [TyObj_name ty_obj, '' '', const_oid_list]"
+   |"str_of_ty OclTy_base_unlimitednatural = ''UnlimitedNatural''"
+   |"str_of_ty OclTy_base_real = ''Real''"
+   |"str_of_ty OclTy_base_string = ''String''"
    |"str_of_ty (OclTy_collection Set ocl_ty) = flatten [''Set('', str_of_ty ocl_ty,'')'']"
    |"str_of_ty (OclTy_collection Sequence ocl_ty) = flatten [''Sequence('', str_of_ty ocl_ty,'')'']"
-   |"str_of_ty (OclTy_raw s) = s"
+   |"str_of_ty (OclTy_raw s) = flatten [unicode_acute, s, unicode_acute]"
 
-definition "ty_boolean = ''Boolean''"
+definition "ty_boolean = str_of_ty OclTy_base_boolean"
+
+fun_quick str_hol_of_ty where
+    "str_hol_of_ty OclTy_base_void = ''unit''"
+   |"str_hol_of_ty OclTy_base_boolean = ''bool''"
+   |"str_hol_of_ty OclTy_base_integer = ''int''"
+   |"str_hol_of_ty OclTy_base_unlimitednatural = ''nat''"
+   |"str_hol_of_ty OclTy_base_real = ''real''"
+   |"str_hol_of_ty OclTy_base_string = ''string''"
+   |"str_hol_of_ty (OclTy_class ty_obj) = flatten [TyObj_name ty_obj, '' '', const_oid_list]"
+   |"str_hol_of_ty (OclTy_raw s) = s"
 
 definition "print_infra_type_synonym_class_set_name name = ''Set_'' @@ name"
 
 fun_quick print_ctxt_ty where
    "print_ctxt_ty c = (\<lambda> OclTy_collection Set t \<Rightarrow> print_infra_type_synonym_class_set_name (print_ctxt_ty t)
                        | OclTy_raw t \<Rightarrow> t
+                       | OclTy_base_void \<Rightarrow> str_of_ty c
                        | OclTy_base_boolean \<Rightarrow> str_of_ty c
-                       | OclTy_base_integer \<Rightarrow> str_of_ty c) c"
+                       | OclTy_base_integer \<Rightarrow> str_of_ty c
+                       | OclTy_base_unlimitednatural \<Rightarrow> str_of_ty c
+                       | OclTy_base_real \<Rightarrow> str_of_ty c
+                       | OclTy_base_string \<Rightarrow> str_of_ty c) c"
 
 fun_quick get_class_hierarchy_strict_aux where
    "get_class_hierarchy_strict_aux dataty l_res =
